\documentclass[uplatex,a4j,12pt,dvipdfmx]{jsarticle}
\usepackage[english]{babel}
\usepackage[letterpaper,top=2cm,bottom=2cm,left=3cm,right=3cm,marginparwidth=1.75cm]{geometry}
\usepackage{amsmath,amsthm,amssymb,bm,color,mathrsfs}
\usepackage{epic,eepic,here}
\usepackage{graphicx}
\title{The Values of the Riemann Zeta Function at Negative Integers}
\author{Masaru Okada}
\date{\today}
\begin{document}
\allowdisplaybreaks
\maketitle

\begin{abstract}
	A memo on the topic of the divergent infinite series $1+2+3+\cdots$ which is known to be represented as the finite value $-1/12$ via analytic continuation. Still in progress.
\end{abstract}

\section{Problem}

For a complex number $s$, the Riemann zeta function (hereafter, simply the zeta function) defined for ${\rm Re}(s) > 1$ is given by
\begin{eqnarray}
	\zeta(s)
	&=&
	1
	+
	\dfrac{1}{2^{s}}
	+
	\dfrac{1}{3^{s}}
	+
	\cdots
	+
	\dfrac{1}{n^{s}}
	+
	\cdots
	\ = \
	\sum_{n=1}^{\infty}
	\dfrac{1}{n^{s}}
\end{eqnarray}

It is clear that the function converges for ${\rm Re}(s) > 1$.
At $s=1$, it becomes the harmonic series and diverges.
However, it can be analytically continued to ${\rm Re}(s) < 0$ by using the following functional equation:
\begin{eqnarray}
	\zeta(s)
	&=&
	2^{s}
	\pi^{s-1}
	{\rm sin}
	\left(
	\dfrac{\pi s}{2}
	\right)
	\ \!
	\Gamma(1-s)
	\zeta(1-s)
	\label{eqn:1302112125}
\end{eqnarray}

\subsection{At $s=-1$}

What about $\zeta(s)$ when $s$ takes a negative value? For example, when $s=-1$,
\begin{eqnarray}
	\zeta(-1)
	&=&
	1
	+
	\dfrac{1}{2^{-1}}
	+
	\dfrac{1}{3^{-1}}
	+
	\cdots
	+
	\dfrac{1}{n^{-1}}
	+
	\cdots
	\nonumber \\[3mm] &=&
	1+2+3+\cdots+n+\cdots
\end{eqnarray}
This can be expressed as an infinite sum that, of course, seems to diverge.
On the other hand, using the functional equation (\ref{eqn:1302112125}) used for analytic continuation,
\begin{eqnarray}
	\zeta(-1)
	&=&
	2^{-1}
	\pi^{-2}
	{\rm sin}
	\left(
	\frac{- \pi}{2}
	\right)
	\ \!
	\Gamma(2)
	\ \!
	\zeta(2)
	\nonumber \\ &=&
	\frac{1}{2 \pi^{2}}
	\times
	(-1)
	\times
	(1!)
	\times
	\frac{\pi^{2}}{6}
	\nonumber \\[3mm] &=&
	- \frac{1}{12}
\end{eqnarray}
The value remains finite. It seems as if these equations suggest a contradiction.

\section{Bernoulli number}

As a preparation, let's briefly summarize Bernoulli numbers $B_{n}$.
$B_{n}$ are defined as the coefficients of the series expansion of the following function:
\begin{eqnarray}
	\dfrac{x}{e^{x}-1}
	&=&
	\sum_{n=0}^{\infty}
	B_{n}
	\dfrac{x^{n}}{n!}
\end{eqnarray}
The general term is also known and is given by
\begin{eqnarray}
	B_{n}
	&=&
	\sum_{k=0}^{n}
	(-1)^{k}
	k^{n}
	\sum_{m=k}^{n}
	\dfrac{{_{m}}{\rm C}_{r}}{m+1}
\end{eqnarray}




Here, the binomial coefficient is denoted as
\begin{eqnarray}
	{_{n}}{\rm C}_{k}
	&=&
	\dfrac{n!}{(n-k)!k!}
\end{eqnarray}
However, since it is a double series, using this formula directly can make the calculation heavy.
Therefore, to actually find $B_{n}$, the following recurrence relation is used:
\begin{eqnarray}
	\left\{
	\begin{array}{l}
		\\
		B_{0} = 1 \\
		B_{0} = -\dfrac{1}{n+1} \displaystyle \sum_{k=0}^{n-1} {_{n+1}}{\rm C}_{k} B_{k}
	\end{array}
	\right.
\end{eqnarray}

All $B_{n}$ are rational numbers. The first few terms are:
$B_{0}=1$, $B_{1}=-\dfrac{1}{2}$, and $B_{2}=\dfrac{1}{6}$.
However, as $n$ gets larger, the numerator and denominator of $B_{n}$ become large, making them unsuitable for floating-point arithmetic.
For example,
$B_{24}=-\dfrac{236364091}{2730}$,
$B_{28}=-\dfrac{1869628555}{58}$.

It is also known that $B_{n}=0$ for odd $n \geq 3$ (all odd $n$ except for $n=1$).
This can be proven as follows:
\begin{eqnarray}
	\dfrac{x}{e^{x}-1}
	-
	B_{1}
	\dfrac{x^{1}}{1!}
	&=&
	\dfrac{x}{e^{x}-1}
	+
	\dfrac{1}{2}x
	\nonumber \\ &=&
	\dfrac{2x + x(e^{x} -1)}{2(e^{x}-1)}
	\nonumber \\ &=&
	\dfrac{x}{2}
	\dfrac{(e^{x} +1) \times e^{-x/2}}{(e^{x}-1)\times e^{-x/2}}
	\nonumber \\ &=&
	\dfrac{x}{2}
	{\rm coth}\dfrac{x}{2}
\end{eqnarray}
Since the ${\rm coth}$ function is an odd function, the expression above becomes an even function.
Therefore, when we expand the above expression as a series, only terms of even powers remain.
That is,
$B_{n}=0$ for odd $n \geq 3$ (all odd $n$ except for $n=1$).

\subsection{Series expansion of coth}

Solving in reverse,
\begin{eqnarray}
	{\rm coth}x
	&=&
	\dfrac{2}{2x}
	\left(
	-
	B_{1}
	\dfrac{(2x)^{1}}{1!}
	+
	\dfrac{2x}{e^{2x}-1}
	\right)
	\nonumber \\ &=&
	\dfrac{1}{x}
	\left(
	-B_{1}(2x)
	+
	\sum_{n=0}^{\infty}
	B_{n}
	\dfrac{(2x)^{n}}{n!}
	\right)
	\nonumber \\ &=&
	\dfrac{1}{x}
	\left(
	-B_{1}(2x)
	+
	B_{0}
	+
	(2x)
	B_{1}
	+
	\dfrac{1}{2!}
	(2x)^{2}
	B_{2}
	+
	\dfrac{1}{3!}
	(2x)^{3}
	B_{3}
	+
	\cdots
	+
	\dfrac{1}{n!}
	(2x)^{n}
	B_{n}
	+
	\cdots
	\right)
	\nonumber \\ &=&
	\dfrac{1}{x}
	\left(
	B_{0}
	+
	\dfrac{1}{2!}
	(2x)^{2}
	B_{2}
	+
	\dfrac{1}{3!}
	(2x)^{3}
	B_{3}
	+
	\cdots
	+
	\dfrac{1}{n!}
	(2x)^{n}
	B_{n}
	+
	\cdots
	\right)
	\label{eqn:1302100637nemui}
\end{eqnarray}
$B_{0}=1$. Furthermore, since $B_{n}=0$ for odd $n \geq 3$,
\begin{eqnarray}
	{\rm eqn.}(\ref{eqn:1302100637nemui})
	&=&
	\dfrac{1}{x}
	\left(
	1
	+
	\dfrac{1}{2!}
	(2x)^{2}
	B_{2}
	+
	\dfrac{1}{4!}
	(2x)^{4}
	B_{4}
	+
	\cdots
	+
	\dfrac{1}{(2n)!}
	(2x)^{2n}
	B_{2n}
	+
	\cdots
	\right)
	\nonumber \\ &=&
	\dfrac{1}{x}
	+
	\sum_{n=1}^{\infty}
	\dfrac{
		2^{2n}
		B_{2n}
	}{(2n)!}
	x^{2n-1}
\end{eqnarray}




\subsection{Series expansion of cot}
\begin{eqnarray}
	{\rm coth} \ \! x
	\ = \
	\dfrac{{\rm cosh} \ \! x}{{\rm sinh} \ \! x}
	\ = \
	\dfrac{{\rm cos}(ix)}{-i{\rm sin}(ix)}
	\ = \
	i {\rm cot} (ix)
\end{eqnarray}
Therefore, substituting $ix \to y$,
\begin{eqnarray}
	{\rm cot} \ \! y
	&=&
	\dfrac{1}{i} {\rm coth} \dfrac{y}{i}
	\ = \
	-i {\rm coth} (-iy)
	\nonumber \\ &=&
	i {\rm coth} (iy)
	\nonumber \\ &=&
	i
	\left\{
	\dfrac{1}{iy}
	+
	\left(
	\dfrac{1}{2!}
	2^{2} (iy)^{1}
	B_{2}
	+
	\dfrac{1}{4!}
	2^{4} (iy)^{3}
	B_{4}
	+
	\cdots
	+
	\dfrac{1}{(2n)!}
	2^{2n} (iy)^{2n-1}
	B_{2n}
	+
	\cdots
	\right)
	\right\}
	\nonumber \\ &=&
	\dfrac{1}{y}
	+
	\sum_{n=1}^{\infty}
	\dfrac{(-1)^{n} 2^{2n} B_{2n} }{(2n)!}
	y^{2n-1}
\end{eqnarray}

\subsection{Series expansion of tan}

Taking the reciprocal of both sides of the double-angle formula
\begin{eqnarray}
	{\rm tan} (2x)
	&=&
	\dfrac{ 2 {\rm tan} \ \! x }{ 1 - {\rm tan}^{2} \ \! x }
\end{eqnarray}
we get
\begin{eqnarray}
	{\rm cot} (2x)
	&=&
	\dfrac{ 1 - {\rm tan}^{2} \ \! x }{2 {\rm tan} \ \! x }
	\nonumber \\ &=&
	\dfrac{1}{2 {\rm tan} \ \! x }
	-
	\dfrac{{\rm tan} \ \! x}{2}
\end{eqnarray}
That is,
\begin{eqnarray}
	{\rm tan} \ \! x
	&=&
	{ \rm cot } \ \! x
	-
	2 { \rm cot } (2x)
	\nonumber \\[2mm] &=&
	\dfrac{1}{x}
	+
	\sum_{n=1}^{\infty}
	\dfrac{(-1)^{n} 2^{2n} B_{2n} }{(2n)!}
	x^{2n-1}
	-
	2
	\left(
	\dfrac{1}{2x}
	+
	\sum_{n=1}^{\infty}
	\dfrac{(-1)^{n} 2^{2n} B_{2n} }{(2n)!}
		(2x)^{2n-1}
	\right)
	\nonumber \\ &=&
	\sum_{n=1}^{\infty}
	\dfrac{(-1)^{n} 2^{2n} B_{2n} }{(2n)!}
	\Big\{
	x^{2n-1}
	-
	2
	(2x)^{2n-1}
	\Big\}
	\nonumber \\ &=&
	\sum_{n=1}^{\infty}
	\dfrac{(-1)^{n} 2^{2n} ( 1 - 2^{2n} ) B_{2n} }{(2n)!}
	x^{2n-1}
\end{eqnarray}
Thus, it is clear that $B_{n}$ are basically involved in the series expansion coefficients of trigonometric functions.
As for the sin and cos functions,
\begin{eqnarray}
	{\rm sin} \ \! x
	&=&
	\dfrac{e^{ix} - e^{-ix}}{2i}
	\\
	{\rm cos} \ \! x
	&=&
	\dfrac{e^{ix} + e^{-ix}}{2}
\end{eqnarray}
The exponential functions are only in the numerator, not in the denominator, so $B_{n}$ does not appear.




\section{Some special cases}

The value of $\zeta(s)$ for a general $s$ is calculated numerically.
However, for special values of $s$, the analytic values are known to be as follows.

For any positive even integer $2m$,
\begin{eqnarray}
	\zeta(2m)
	&=&
	\dfrac{(-1)^{2m} B_{2m} (2 \pi)^{2m} }{(2m)! 2}
\end{eqnarray}

For any negative integer $-m$,
\begin{eqnarray}
	\zeta(-m)
	&=&
	-
	\dfrac{B_{m+1}}{m+1}
\end{eqnarray}

There is no known elementary expression for the value of $\zeta(s)$ when $s$ is an odd number.
However, a series representation was given by Ramanujan.
For any odd number $2m-1$,
\begin{eqnarray}
	\zeta(2m-1)
	&=&
	-
	2^{2m} \pi^{2m-1}
	\sum_{k=0}^{m}
	(-1)^{k+1}
	\dfrac{B_{2k}}{(2k)!2}
	\dfrac{B_{2m-2k}}{(2m-2k)!}
	-
	2
	\sum_{k=1}^{\infty}
	\dfrac{ k^{-2m+1} }{ e^{2 \pi k} - 1 }
\end{eqnarray}

${}$

${}$

${}$

\section{Analytic continuation}

In the Gamma function
\begin{eqnarray}
	\Gamma(s)
	&=&
	\int^{\infty}_{0}
	\!\! dt
	\ \! t^{s-1} e^{-t}
\end{eqnarray}
by changing the variable to $t=nx$, we get
\begin{eqnarray}
	\Gamma(s)
	&=&
	\int^{\infty}_{0}
	\!\! ndx
	\ \! (nx)^{s-1} e^{-nx}
	\label{eqn:1302120225hayonena}
\end{eqnarray}
Furthermore, by dividing both sides by $n^{s}$ and taking the sum over all natural numbers $n$,
\begin{eqnarray}
	\sum_{n=1}^{\infty}
	\dfrac{ \Gamma(s) }{ n^{s} }
	&=&
	\sum_{n=1}^{\infty}
	\int^{\infty}_{0}
	\!\! dx
	\ \! x^{s-1} e^{-nx}
	\nonumber \\
	\Gamma(s)
	\sum_{n=1}^{\infty}
	\dfrac{ 1 }{ n^{s} }
	&=&
	\int^{\infty}_{0}
	\!\! dx
	\ \! x^{s-1}
	\sum_{n=1}^{\infty}
	e^{-nx}
\end{eqnarray}
Thus, the expression
\begin{eqnarray}
	\Gamma(s)
	\zeta(s)
	&=&
	\int^{\infty}_{0}
	\!\! dx
	\ \!
	\dfrac{x^{s-1}}{e^{x} - 1}
	\label{eqn:1302120248nerana}
\end{eqnarray}
is obtained.




By the way, using the following identity for alternating series
\begin{eqnarray}
	1
	-
	\dfrac{1}{2^{s}}
	+
	\dfrac{1}{3^{s}}
	-
	\cdots
	+
	\dfrac{(-1)^{n+1}}{n^{s}}
	+
	\cdots
	&=&
	\left\{
	1
	+
	\dfrac{1}{2^{s}}
	+
	\dfrac{1}{3^{s}}
	+
	\cdots
	+
	\dfrac{1}{n^{s}}
	+
	\cdots
	\right\}
	-
	2
	\left\{
	\dfrac{1}{2^{s}}
	+
	\dfrac{1}{4^{s}}
	+
	\cdots
	+
	\dfrac{1}{(2n)^{s}}
	+
	\cdots
	\right\}
	\nonumber \\
	\sum_{n=1}^{\infty}
	\dfrac{(-1)^{n+1}}{n^{s}}
	&=&
	\zeta(s)
	-
	2
	\sum_{n=1}^{\infty}
	\dfrac{1}{(2n)^{s}}
	\nonumber \\ &=&
	\zeta(s)
	-
	\dfrac{2}{2^{s}}
	\zeta(s)
	\nonumber \\ &=&
	\zeta(s)
	\left(
	1
	-
	\dfrac{1}{2^{s-1}}
	\right)
\end{eqnarray}
and equation (\ref{eqn:1302120225hayonena}), if we calculate the right and left sides independently,
\begin{eqnarray}
	\sum_{n=1}^{\infty}
	\Gamma(s)
	\dfrac{(-1)^{n+1}}{n^{s}}
	&=&
	\sum_{n=1}^{\infty}
	\left\{
	\int^{\infty}_{0}
	\!\! ndx
	\ \! (nx)^{s-1} e^{-nx}
	\right\}
	\dfrac{(-1)^{n+1}}{n^{s}}
	\nonumber \\
	\Gamma(s)
	\sum_{n=1}^{\infty}
	\dfrac{(-1)^{n+1}}{n^{s}}
	&=&
	\int^{\infty}_{0}
	\!\! dx
	\ \! x^{s-1}
	\sum_{n=1}^{\infty}
	(-1)^{n+1}
	e^{-nx}
	\nonumber \\
	\Gamma(s)
	\zeta(s)
	\left(
	1
	-
	\dfrac{1}{2^{s-1}}
	\right)
	&=&
	\int^{\infty}_{0}
	\!\! dx
	\ \! x^{s-1}
	\frac{1}{e^{x} + 1}
\end{eqnarray}
is newly obtained.

${}$

From equation (\ref{eqn:1302120225hayonena}),
\begin{eqnarray}
	\dfrac{1}{n^{s}}
	&=&
	\dfrac{1}{\Gamma(s)}
	\int^{\infty}_{0}
	dt \ \! t^{s-1} e^{-nt}
\end{eqnarray}
Using this fact,
\begin{eqnarray}
	\pi^{-s/2}
	\zeta(s)
	&=&
	\sum_{n=1}^{\infty}
	\dfrac{1}{(\pi n )^{s/2}}
	\nonumber \\ &=&
	\sum_{n=1}^{\infty}
	\dfrac{1}{\Gamma(s/2)}
	\int^{\infty}_{0}
	dt \ \! t^{s/2 \ \! -1} e^{-(\pi n^{2})t}
	\nonumber \\ &=&
	\dfrac{1}{\Gamma(s/2)}
	\int^{\infty}_{0}
	dt \ \! t^{s/2 \ \! -1}
	\sum_{n=1}^{\infty}
	e^{- \pi n^{2} t}
\end{eqnarray}

Here, as a special case of the Jacobi theta function, we define $\psi(x)$ as
\begin{eqnarray}
	\psi(x)
	&=&
	\sum_{n=1}^{\infty}
	e^{- \pi n^{2} x}
\end{eqnarray}
From the Poisson summation formula,
$\psi(x)$ satisfies the following.
\begin{eqnarray}
	2 \psi ( 1/x )
	+
	1
	&=&
	\sqrt{x}
	\Big( 2 \psi(x) + 1 \Big)
\end{eqnarray}

\ \\

(The following is still being written...)

\end{document}